\begin{frame}

\frametitle{The syntax of \D{}}

\setcounter{equation}{0}

\begin{align*}
\nonterm{program}\ \textt{::=}&\ \nonterm{clause}^{\color{red}\textt{+}}
\ \nonterm{expression}
& \\
\nonterm{expression}\ \textt{::=}&\ \nonterm{element}\ \textt{(}\ \term{.}
\ \nonterm{expression}\ \textt{)}\ \textt{?}
& x\\
\nonterm{element}\ \textt{::=}&\ \term{0}\ \textt{|}\ \term{(}
\ \nonterm{element}\ \term{)}\ \textt{|}\ \nonterm{name}\ \textt{|}
\ \nonterm{application}
& e\\
\nonterm{application}\ \textt{::=}&\ \nonterm{name}
\ \nonterm{expression}^{\color{yellow}\textt{*}}
& \left\langle v,X \right\rangle \\
\nonterm{clause}\ \textt{::=}&\ \nonterm{name}
\ \nonterm{pattern}^{\color{yellow}\textt{*}}\ \term{:=}
\ \nonterm{expression}
& c=\left\langle v, P, x \right\rangle \\
\nonterm{pattern}\ \textt{::=}&\ \nonterm{pattern-element}\ \textt{(}
\ \term{.}\ \nonterm{pattern}\ \textt{)}\ \textt{?}
& p\\
\nonterm{pattern-element}\ \textt{::=}&\ \term{0}\ \textt{|}\ \term{\_}
\ \textt{|}\ \term{(}\ \nonterm{pattern}\ \term{)}\ \textt{|}\ \nonterm{name}
& p\\
\nonterm{name}\ \textt{::=}&\ \textt{[}\term{a}\mathmono{-}\term{z}\textt{]}
\ \textt{(}\ \textt{[}\term{-}\ \term{a}\mathmono{-}\term{z}\textt{]}^\textt{*}
\ \textt{[}\term{a}\mathmono{-}\term{z}\textt{]}\ \textt{)}\ \textt{?}
& v
\end{align*}

(14)

% e in this case could've well been x.. %

\end{frame}
